doc/examples/interp.lean
@@ -1,7 +1,5 @@
 /-|
-==========================================
-The Well-Typed Interpreter
-==========================================
+# The Well-Typed Interpreter
 
 In this example, we build an interpreter for a simple functional programming language,
 with variables, function application, binary operators and an `if...then...else` construct.
@@ -22,7 +20,7 @@ inductive Vector (α : Type u) : Nat → Type u
   | cons : α → Vector α n → Vector α (n+1)
 
 /-|
-We can overload the `List.cons` notation `::` and use it to create `Vector`\ s.
+We can overload the `List.cons` notation `::` and use it to create `Vector`s.
 -/
 infix:67 " :: " => Vector.cons
 
@@ -133,7 +131,7 @@ We can make some simple test functions. Firstly, adding two inputs `fun x y => y
 -/
 
 def add : Expr ctx (Ty.fn Ty.int (Ty.fn Ty.int Ty.int)) :=
-  lam (lam (op (.+.) (var stop) (var (pop stop))))
+  lam (lam (op (·+·) (var stop) (var (pop stop))))
 
 #eval add.interp Env.nil 10 20
 
@@ -146,9 +144,9 @@ definition itself is non-terminating. We use two tricks to make sure Lean accept
 -/
 
 def fact : Expr ctx (Ty.fn Ty.int Ty.int) :=
-  lam (ife (op (.==.) (var stop) (val 0))
+  lam (ife (op (·==·) (var stop) (val 0))
            (val 1)
-           (op (.*.) (delay fun _ => app fact (op (.-.) (var stop) (val 1))) (var stop)))
+           (op (·*·) (delay fun _ => app fact (op (·-·) (var stop) (val 1))) (var stop)))
   decreasing_by sorry
 
 #eval fact.interp Env.nil 10
